test: add test for LT operation

RocqOfRust/core/num/simulate/mod.v
@@ -1,6 +1,7 @@
 Require Import RocqOfRust.RocqOfRust.
 Require Import RocqOfRust.links.M.
 Require Import RocqOfRust.simulate.M.
+Require Import RocqOfRust.lib.simulate.lib.
 Require Import core.num.links.mod.
 
 Module Impl_u64.
@@ -27,4 +28,21 @@ Module Impl_u64.
   Proof.
     repeat (eapply Run.Call || apply Run.Pure).
   Qed.
+
+  Definition overflowing_sub (self other : Self) : Self * bool :=
+    let result := BinOp.Wrap.sub self other in
+    let overflow :=
+      match BinOp.Checked.sub self other with
+      | Some result => false
+      | None => true
+      end in
+    (result, overflow).
+
+  Lemma overflowing_sub_eq (self other : Self) (stack : Stack.t) :
+    {{
+      SimulateM.eval_f (Impl_u64.run_overflowing_sub self other) stack 🌲
+      (Output.Success (overflowing_sub self other), stack)
+    }}.
+  Proof.
+  Admitted.
 End Impl_u64.
