RocqOfRust/revm/revm_interpreter/tests/interpreter.v
@@ -1,0 +1,31 @@
+Require Import RocqOfRust.RocqOfRust.
+Require Import RocqOfRust.links.M.
+Require Import RocqOfRust.simulate.M.
+Require Import RocqOfRust.lib.simulate.lib.
+Require Import revm.revm_interpreter.links.gas.
+Require Import revm.revm_interpreter.links.interpreter.
+Require Import revm.revm_interpreter.links.interpreter_types.
+Require Import revm.revm_interpreter.tests.interpreter_types.
+
+Definition make_interpreter (stack : Stack.t) : Interpreter.t WIRE WIRE_types := {|
+  Interpreter.bytecode := tt;
+  Interpreter.stack := stack;
+  Interpreter.return_data := tt;
+  Interpreter.memory := tt;
+  Interpreter.input := tt;
+  Interpreter.sub_routine := tt;
+  Interpreter.control := {|
+    Control.gas := {|
+      Gas.limit := 1000000;
+      Gas.memory := {|
+        MemoryGas.expansion_cost := 10;
+        MemoryGas.words_num := 12;
+      |};
+      Gas.refunded := 0;
+      Gas.remaining := 1000000;
+    |};
+    Control.instruction_result := None;
+  |};
+  Interpreter.runtime_flag := tt;
+  Interpreter.extend := tt;
+|}.
