RocqOfRust/revm/revm_interpreter/tests/interpreter_types.v
@@ -1,0 +1,277 @@
+Require Import RocqOfRust.RocqOfRust.
+Require Import RocqOfRust.links.M.
+Require Import RocqOfRust.simulate.M.
+Require Import RocqOfRust.lib.simulate.lib.
+Require Import alloy_primitives.bits.links.address.
+Require Import alloy_primitives.bits.links.fixed.
+Require Import alloy_primitives.bytes.links.mod.
+Require Import alloy_primitives.links.aliases.
+Require Import core.links.array.
+Require Import core.ops.links.range.
+Require Import revm.revm_bytecode.eof.links.types_section.
+Require Import revm.revm_interpreter.links.gas.
+Require Import revm.revm_interpreter.links.instruction_result.
+Require Import revm.revm_interpreter.links.interpreter_action.
+Require Import revm.revm_interpreter.links.interpreter_types.
+Require Import revm.revm_interpreter.simulate.interpreter_types.
+Require Import revm.revm_specification.links.hardfork.
+Require Import ruint.links.lib.
+
+Parameter WIRE : Set.
+
+Instance Link_WIRE : Link WIRE.
+Admitted.
+
+Module Stack.
+  (** Note: we represent the list in reverse order to simplify access to the top in patterns *)
+  Record t : Set := {
+    value : list aliases.U256.t;
+  }.
+
+  Instance IsLink : Link t.
+  Admitted.
+End Stack.
+Export (hints) Stack.
+
+Module Control.
+  Record t : Set := {
+    gas : Gas.t;
+    instruction_result : option InstructionResult.t;
+  }.
+
+  Instance IsLink : Link t.
+  Admitted.
+End Control.
+Export (hints) Control.
+
+Definition WIRE_types : InterpreterTypes.Types.t := {|
+  InterpreterTypes.Types.Stack := Stack.t;
+  InterpreterTypes.Types.Memory := unit;
+  InterpreterTypes.Types.Memory_Synthetic := unit;
+  InterpreterTypes.Types.Memory_Synthetic1 := unit;
+  InterpreterTypes.Types.Bytecode := unit;
+  InterpreterTypes.Types.ReturnData := unit;
+  InterpreterTypes.Types.Input := unit;
+  InterpreterTypes.Types.SubRoutineStack := unit;
+  InterpreterTypes.Types.Control := Control.t;
+  InterpreterTypes.Types.RuntimeFlag := unit;
+  InterpreterTypes.Types.Extend := unit;
+|}.
+
+Instance AreLinks_WIRE_types : InterpreterTypes.Types.AreLinks WIRE_types := {}.
+
+Module Immediates.
+  Instance I : Immediates.C WIRE_types.(InterpreterTypes.Types.Bytecode).
+  Admitted.
+End Immediates.
+Export (hints) Immediates.
+
+Module LegacyBytecode.
+  Instance I : LegacyBytecode.C WIRE_types.(InterpreterTypes.Types.Bytecode).
+  Admitted.
+End LegacyBytecode.
+Export (hints) LegacyBytecode.
+
+Module Jumps.
+  Instance I : Jumps.C WIRE_types.(InterpreterTypes.Types.Bytecode).
+  Admitted.
+End Jumps.
+Export (hints) Jumps.
+
+Module EofData.
+  Instance I : EofData.C WIRE_types.(InterpreterTypes.Types.Bytecode).
+  Admitted.
+End EofData.
+Export (hints) EofData.
+
+Module EofContainer.
+  Instance I : EofContainer.C WIRE_types.(InterpreterTypes.Types.Bytecode).
+  Admitted.
+End EofContainer.
+Export (hints) EofContainer.
+
+Module EofCodeInfo.
+  Instance I : EofCodeInfo.C WIRE_types.(InterpreterTypes.Types.Bytecode).
+  Admitted.
+End EofCodeInfo.
+Export (hints) EofCodeInfo.
+
+Module InputTraits.
+  Instance I : InputTraits.C WIRE_types.(InterpreterTypes.Types.Input).
+  Admitted.
+End InputTraits.
+Export (hints) InputTraits.
+
+Module StackTrait.
+  Definition Self : Set :=
+    Stack.t.
+
+  Definition len (self : Self) : usize :=
+    Z.of_nat (List.length self.(Stack.value)).
+
+  Definition is_empty (self : Self) : bool :=
+    match self.(Stack.value) with
+    | [] => true
+    | _ => false
+    end.
+
+  (* TODO: check spec *)
+  Definition push (self : Self) (value : aliases.U256.t) : bool * Self :=
+    let MAX_LEN := Z.of_nat 1024 in
+    if i[len self] <=? MAX_LEN then
+      (true, self <| Stack.value := value :: self.(Stack.value) |>)
+    else
+      (false, self).
+
+  Definition push_b256 (self : Self) (value : aliases.B256.t) : bool * Self.
+  Admitted.
+
+  (* TODO: check spec: do we let the stack as empty if the stack is too short? *)
+  Fixpoint popn_nat (N : nat) (self : Self) : option (ArrayPairs.t aliases.U256.t N) * Self :=
+    match N with
+    | O => (Some ArrayEmpty.Make, self)
+    | S N =>
+      match self.(Stack.value) with
+      | [] => (None, self)
+      | value :: rest =>
+        let '(result, self') := popn_nat N (self <| Stack.value := rest |>) in
+        match result with
+        | Some values => (Some {| ArrayPair.x := value; ArrayPair.xs := values |}, self')
+        | None => (None, self')
+        end
+      end
+    end.
+
+  Definition popn (N : usize) (self : Self) : option (array.t aliases.U256.t N) * Self :=
+    let '(result, self') := popn_nat (Z.to_nat i[N]) self in
+    match result with
+    | Some values => (Some {| array.value := values |}, self')
+    | None => (None, self')
+    end.
+
+  Definition top (self : Self) : option (RefStub.t Self aliases.U256.t) :=
+    match self.(Stack.value) with
+    | [] => None
+    | default_value :: _ =>
+      Some {|
+        RefStub.path := [];
+        RefStub.projection x :=
+          match x.(Stack.value) with
+          | [] => default_value (* impossible *)
+          | value :: _ => value
+          end;
+        RefStub.injection x value :=
+          match x.(Stack.value) with
+          | [] => {| Stack.value := [] |} (* impossible *)
+          | _ :: rest => {| Stack.value := value :: rest |}
+          end;
+      |}
+    end.
+
+  Definition popn_top (N : usize) (self : Self) :
+      option (array.t aliases.U256.t N * RefStub.t Self aliases.U256.t) * Self :=
+    let '(result, self') := popn N self in
+    match result with
+    | Some values =>
+      let top_stub := top self' in
+      match top_stub with
+      | Some top_stub => (Some (values, top_stub), self')
+      | None => (None, self')
+      end
+    | None => (None, self')
+    end.
+
+  Definition pop (self : Self) : option aliases.U256.t * Self.
+  Admitted.
+
+  Definition pop_address (self : Self) : option Address.t * Self.
+  Admitted.
+
+  Definition exchange (self : Self) (n m : usize) : bool * Self.
+  Admitted.
+
+  Definition dup (self : Self) (n : usize) : bool * Self.
+  Admitted.
+
+  Instance I : StackTrait.C WIRE_types.(InterpreterTypes.Types.Stack) := {
+    StackTrait.len := len;
+    StackTrait.is_empty := is_empty;
+    StackTrait.push := push;
+    StackTrait.push_b256 := push_b256;
+    StackTrait.popn := popn;
+    StackTrait.popn_top := popn_top;
+    StackTrait.top := top;
+    StackTrait.pop := pop;
+    StackTrait.pop_address := pop_address;
+    StackTrait.exchange := exchange;
+    StackTrait.dup := dup;
+  }.
+End StackTrait.
+Export (hints) StackTrait.
+
+Module LoopControl.
+  Definition Self : Set :=
+    Control.t.
+
+  Definition set_instruction_result (self : Self) (result : InstructionResult.t) : Self :=
+    self <| Control.instruction_result := Some result |>.
+
+  Definition set_next_action
+      (self : Self)
+      (action : InterpreterAction.t)
+      (result : InstructionResult.t) :
+      Self.
+  Admitted.
+
+  Definition gas : RefStub.t Self Gas.t := {|
+    RefStub.path := [];
+    RefStub.projection := fun x => x.(Control.gas);
+    RefStub.injection := fun x y => x <| Control.gas := y |>;
+  |}.
+
+  Definition instruction_result (self : Self) : InstructionResult.t.
+  Admitted.
+
+  Definition take_next_action (self : Self) : InterpreterAction.t * Self.
+  Admitted.
+
+  Instance I : LoopControl.C WIRE_types.(InterpreterTypes.Types.Control) := {|
+    simulate.interpreter_types.LoopControl.set_instruction_result := set_instruction_result;
+    simulate.interpreter_types.LoopControl.set_next_action := set_next_action;
+    simulate.interpreter_types.LoopControl.gas := gas;
+    simulate.interpreter_types.LoopControl.instruction_result := instruction_result;
+    simulate.interpreter_types.LoopControl.take_next_action := take_next_action;
+  |}.
+End LoopControl.
+Export (hints) LoopControl.
+
+Module RuntimeFlag.
+  Instance I : RuntimeFlag.C WIRE_types.(InterpreterTypes.Types.RuntimeFlag).
+  Admitted.
+End RuntimeFlag.
+Export (hints) RuntimeFlag.
+
+Module MemoryTrait.
+  Instance I : MemoryTrait.C WIRE_types.(InterpreterTypes.Types.Memory)
+    WIRE_types.(InterpreterTypes.Types.Memory_Synthetic)
+    WIRE_types.(InterpreterTypes.Types.Memory_Synthetic1).
+  Admitted.
+End MemoryTrait.
+Export (hints) MemoryTrait.
+
+Module SubRoutineStack.
+  Instance I : SubRoutineStack.C WIRE_types.(InterpreterTypes.Types.SubRoutineStack).
+  Admitted.
+End SubRoutineStack.
+Export (hints) SubRoutineStack.
+
+Module ReturnData.
+  Instance I : ReturnData.C WIRE_types.(InterpreterTypes.Types.ReturnData).
+  Admitted.
+End ReturnData.
+Export (hints) ReturnData.
+
+Module InterpreterTypes.
+  Instance I : InterpreterTypes.C WIRE_types := {}.
+End InterpreterTypes.
+Export (hints) InterpreterTypes.
